theories/Handlers/Mutex.v
@@ -27,17 +27,17 @@ Section defs.
 
   Let TE := @TraceElem PID req_t ret_t.
 
-  Inductive mutex_chain_rule : state_t -> state_t -> TE -> Prop :=
+  Inductive mutex_state_transition : state_t -> state_t -> TE -> Prop :=
   | mutex_grab : forall pid,
-      mutex_chain_rule None (Some pid) (trace_elem pid grab I)
+      mutex_state_transition None (Some pid) (trace_elem pid grab I)
   | mutex_release_ok : forall pid,
-      mutex_chain_rule (Some pid) None (trace_elem pid release true)
+      mutex_state_transition (Some pid) None (trace_elem pid release true)
   | mutex_release_fail : forall pid,
-      mutex_chain_rule None None (trace_elem pid release false).
+      mutex_state_transition None None (trace_elem pid release false).
 
   Global Instance mutexHandler : @Handler PID req_t ret_t :=
     { h_state := state_t;
-      h_chain_rule := mutex_chain_rule;
+      h_state_transition := mutex_state_transition;
     }.
 
   Theorem no_double_grab_0 : forall (a1 a2 : PID),
@@ -64,7 +64,7 @@ End defs.
 
 Ltac mutex_contradiction :=
   match goal with
-    [H1 : mutex_chain_rule _ ?s1 ?s2 _, H2 : mutex_chain_rule _ ?s2 ?s3 _ |- _] =>
+    [H1 : mutex_state_transition _ ?s1 ?s2 _, H2 : mutex_state_transition _ ?s2 ?s3 _ |- _] =>
       inversion H1; inversion H2; subst; discriminate
   end.
 
@@ -72,5 +72,5 @@ Hint Extern 4 => mutex_contradiction : handlers.
 
 Ltac clear_mutex :=
   repeat match goal with
-           [H: mutex_chain_rule _ _ _ _ |- _] => clear H
+           [H: mutex_state_transition _ _ _ _ |- _] => clear H
          end.
